lib/coq/Prompt_monad.v
@@ -69,7 +69,6 @@ Require Import String.
 (*Require Import Sail_impl_base*)
 Require Import Sail.Instr_kinds.
 Require Import Sail.Values.
-Require bbv.Word.
 Import ListNotations.
 Local Open Scope Z.
 
@@ -286,7 +285,7 @@ Definition try_catchR {rv A R E1 E2} (m : monadR rv A R E1) (h : E1 -> monadR rv
 
 (*val read_memt_bytes : forall 'rv 'a 'b 'e. Bitvector 'a, Bitvector 'b => read_kind -> 'a -> integer -> monad 'rv (list memory_byte * bitU) 'e*)
 Definition read_memt_bytes {rv A E} rk (addr : mword A) sz : monad rv (list memory_byte * bitU) E :=
-  Read_memt rk (Word.wordToN (get_word addr)) (Z.to_nat sz) returnm.
+  Read_memt rk (mword_to_N addr) (Z.to_nat sz) returnm.
 
 (*val read_memt : forall 'rv 'a 'b 'e. Bitvector 'a, Bitvector 'b => read_kind -> 'a -> integer -> monad 'rv ('b * bitU) 'e*)
 Definition read_memt {rv A E} rk (addr : mword A) sz : monad rv (mword (8 * sz) * bitU) E :=
@@ -300,7 +299,7 @@ Definition read_memt {rv A E} rk (addr : mword A) sz : monad rv (mword (8 * sz) 
 
 (*val read_mem_bytes : forall 'rv 'a 'b 'e. Bitvector 'a, Bitvector 'b => read_kind -> 'a -> integer -> monad 'rv (list memory_byte) 'e*)
 Definition read_mem_bytes {rv A E} rk (addr : mword A) sz : monad rv (list memory_byte) E :=
-  Read_mem rk (Word.wordToN (get_word addr)) (Z.to_nat sz) returnm.
+  Read_mem rk (mword_to_N addr) (Z.to_nat sz) returnm.
 
 (*val read_mem : forall 'rv 'a 'b 'e. Bitvector 'a, Bitvector 'b => read_kind -> 'a -> integer -> monad 'rv 'b 'e*)
 Definition read_mem {rv A E} rk (addrsz : Z) (addr : mword A) sz : monad rv (mword (8 * sz)) E :=
@@ -315,12 +314,12 @@ Definition excl_result {rv e} (_:unit) : monad rv bool e :=
   Excl_res k.
 
 Definition write_mem_ea {rv a E} wk (addrsz : Z) (addr: mword a) sz : monad rv unit E :=
- Write_ea wk (Word.wordToN (get_word addr)) (Z.to_nat sz) (Done tt).
+ Write_ea wk (mword_to_N addr) (Z.to_nat sz) (Done tt).
 
 (*val write_mem : forall 'rv 'a 'b 'e. Bitvector 'a, Bitvector 'b =>
   write_kind -> integer -> 'a -> integer -> 'b -> monad 'rv bool 'e*)
 Definition write_mem {rv a E} wk (addrsz : Z) (addr : mword a) sz (v : mword (8 * sz)) : monad rv bool E :=
-  match (mem_bytes_of_bits v, Word.wordToN (get_word addr)) with
+  match (mem_bytes_of_bits v, mword_to_N addr) with
     | (Some v, addr) =>
        Write_mem wk addr (Z.to_nat sz) v returnm
     | _ => Fail "write_mem"
@@ -329,19 +328,19 @@ Definition write_mem {rv a E} wk (addrsz : Z) (addr : mword a) sz (v : mword (8 
 (*val write_memt : forall 'rv 'a 'b 'e. Bitvector 'a, Bitvector 'b =>
   write_kind -> 'a -> integer -> 'b -> bitU -> monad 'rv bool 'e*)
 Definition write_memt {rv a E} wk (addr : mword a) sz (v : mword (8 * sz)) tag : monad rv bool E :=
-  match (mem_bytes_of_bits v, Word.wordToN (get_word addr)) with
+  match (mem_bytes_of_bits v, mword_to_N addr) with
     | (Some v, addr) =>
        Write_memt wk addr (Z.to_nat sz) v tag returnm
     | _ => Fail "write_mem"
   end.
 
 Definition write_tag {rv a E} wk (addr : mword a) tag : monad rv bool E :=
-  let addr := Word.wordToN (get_word addr) in
+  let addr := mword_to_N addr in
        Write_tag wk addr tag returnm.
 
 (* This alternate version is used in a few places, but should probably disappear *)
 Definition write_tag_bool {rv a E} (addr : mword a) tag : monad rv bool E :=
-  let addr := Word.wordToN (get_word addr) in
+  let addr := mword_to_N addr in
        Write_tag Write_plain addr (bitU_of_bool tag) returnm.
 
 Definition read_reg {s rv a e} (reg : register_ref s rv a) : monad rv a e :=
